examples/Employee_AnalysisModel_UMLPart_generator_shallow.thy
@@ -90,7 +90,7 @@ Class Galaxy
 End
 *)
 
-Define_int [ 1000, 1200, 1300, 1800, 2600, 2900, 3200, 3500 ]
+Define_base [ 1000, 1200, 1300, 1800, 2600, 2900, 3200, 3500 ]
 
 Instance X\<^sub>P\<^sub>e\<^sub>r\<^sub>s\<^sub>o\<^sub>n1 :: Person = [ salary = 1300 , boss = X\<^sub>P\<^sub>e\<^sub>r\<^sub>s\<^sub>o\<^sub>n2 ]
      and X\<^sub>P\<^sub>e\<^sub>r\<^sub>s\<^sub>o\<^sub>n2 :: Person = [ salary = 1800 , boss = X\<^sub>P\<^sub>e\<^sub>r\<^sub>s\<^sub>o\<^sub>n2 ]
